BigNum.Components.Extra: Add more components

Bignum/Component/Extra.lean
@@ -10,17 +10,51 @@ public import Bignum.Component.Basic
 
 @[expose] public section
 
+/-! # More components -/
+
 set_option autoImplicit false
 
 namespace Bignum.Component
 
-/-- Component for a bit within a bitvector. -/
+/--
+Component for a bit within a bitvector.
+-/
 def bitelement {w : Nat} (i : Fin w) : Component (BitVec w) Bool :=
   ⟨λ bv ↦ bv.getLsb i, λ b bv ↦ BitVec.setLsb bv i b⟩
 
-/-- Component for subwords of a bitvector. -/
+/--
+Component for subwords of a bitvector.
+-/
 def subword {w : Nat} (start len : Nat) :
     Component (BitVec w) (BitVec len) :=
   ⟨BitVec.extractLsb' start len, λ b bv ↦ bv.overwriteLsb' start len b⟩
+
+/--
+Component for the bottom-half of a bitvector.
+-/
+def bottomhalf {w : Nat} : Component (BitVec w) (BitVec (w / 2)) :=
+  subword 0 (w / 2)
+
+/--
+Component for the top-half of a bitvector.
+-/
+def tophalf {w : Nat} : Component (BitVec w) (BitVec (w.succ / 2)) :=
+  subword (w / 2) (w.succ / 2)
+
+/-
+Components for subwords of bitvectors with a specific length.
+-/
+def bottom_256 : Component (BitVec 512) (BitVec 256) := @bottomhalf 512
+def top_256    : Component (BitVec 512) (BitVec 256) := @tophalf 512
+def bottom_128 : Component (BitVec 256) (BitVec 128) := @bottomhalf 256
+def top_128    : Component (BitVec 256) (BitVec 128) := @tophalf 256
+def bottom_64  : Component (BitVec 128) (BitVec 64)  := @bottomhalf 128
+def top_64     : Component (BitVec 128) (BitVec 64)  := @tophalf 128
+def bottom_32  : Component (BitVec 64) (BitVec 32)   := @bottomhalf 64
+def top_32     : Component (BitVec 64) (BitVec 32)   := @tophalf 64
+def bottom_16  : Component (BitVec 32) (BitVec 16)   := @bottomhalf 32
+def top_16     : Component (BitVec 32) (BitVec 16)   := @tophalf 32
+def bottom_8   : Component (BitVec 16) (BitVec 8)    := @bottomhalf 16
+def top_8      : Component (BitVec 16) (BitVec 8)    := @tophalf 16
 
 end Bignum.Component
