BignumTest/ComponentExtra.lean
@@ -23,13 +23,26 @@ namespace bitelementNS
 
 namespace subwordNS
 def bv : BitVec 8 := 0b01001011#8
-example : (Component.subword 0 3).read bv == 0b11#3 := by rfl
-example : (Component.subword 4 1).read bv == 0#1 := by rfl
-example : (Component.subword 0 0).read bv == 0#0 := by rfl
-example : (Component.subword 6 3).read bv == 1#3 := by rfl
-example : (Component.subword 7 3).read bv == 0#3 := by rfl
-example : (Component.subword 100 2).read bv == 0#2 := by rfl
-example : (Component.subword 0 3).write 0 bv == 0b01001000#8 := by rfl
-example : (Component.subword 1 3).write 0b101 bv == 0b01001011#8 := by rfl
-example : (Component.subword 6 4).write 0xf bv == 0b11001011#8 := by rfl
+example : (Component.subword 0 3).read bv = 0b11#3 := by rfl
+example : (Component.subword 4 1).read bv = 0#1 := by rfl
+example : (Component.subword 0 0).read bv = 0#0 := by rfl
+example : (Component.subword 6 3).read bv = 1#3 := by rfl
+example : (Component.subword 7 3).read bv = 0#3 := by rfl
+example : (Component.subword 100 2).read bv = 0#2 := by rfl
+example : (Component.subword 0 3).write 0 bv = 0b01001000#8 := by rfl
+example : (Component.subword 1 3).write 0b101 bv = 0b01001011#8 := by rfl
+example : (Component.subword 6 4).write 0xf bv = 0b11001011#8 := by rfl
+example : Component.bottomhalf.read bv = 0b1011#4 := by rfl
+example : Component.bottomhalf.read 0b11#2 = 0b1#1 := by rfl
+example : Component.bottomhalf.read 0b11#0 = 0b1#0 := by rfl
+example : Component.bottomhalf.write 0xf bv = 0b01001111#8 := by rfl
+example : Component.bottomhalf.write 0xf 0#2 = 1#2 := by rfl
+example : Component.bottomhalf.write 0xf 0#0 = 0#0 := by rfl
+example : Component.tophalf.read bv = 0b0100#4 := by rfl
+example : Component.tophalf.read 0b11#2 = 0b1#1 := by rfl
+example : Component.tophalf.read 0b11#0 = 0b1#0 := by rfl
+example : Component.tophalf.write 0xf bv = 0b11111011#8 := by rfl
+example : Component.tophalf.write 0xf 0#2 = 2#2 := by rfl
+example : Component.tophalf.write 0xf 0#0 = 0#0 := by rfl
+example : Component.tophalf.write 0x0 111#3 = 0b001#3 := by rfl
 end subwordNS
